Try to use pcmpestrm.

coq/gen/esc.c
@@ -175,3 +175,298 @@ n4_sse_html_escape(buffer v16_buf, byteptr v15_ptr, nat v14_m, nat v13_n)
     }
   }
 }
+buffer
+n4_sse_html_escape2_dense(buffer v129_buf,
+                          nat v128_n,
+                          nat v127_mask,
+                          m128 v126_bytes)
+{
+  n4_sse_html_escape2_dense:;
+  switch (sw_nat(v128_n))
+  {
+    case_O_nat: { return v129_buf; }
+    case_S_nat: {
+      nat v131_n_ = field0_S_nat(v128_n);
+      ascii v132_c = n1_m128_firstbyte(v126_bytes);
+      m128 v133_rest = n1_m128_restbytes(v126_bytes);
+      prod_byteptr_nat v134_p = n1_html_escape_byte_table(v132_c);
+      byteptr v135_escptr = field0_pair_prod_byteptr_nat(v134_p);
+      nat v136_escn = field1_pair_prod_byteptr_nat(v134_p);
+      buffer v137_buf_ = n3_bufaddmem(v129_buf, v135_escptr, v136_escn);
+      nat v138_n = n1_half(v127_mask);
+      v129_buf = v137_buf_;
+      v128_n = v131_n_;
+      v127_mask = v138_n;
+      v126_bytes = v133_rest;
+      goto n4_sse_html_escape2_dense;
+    }
+  }
+}
+buffer
+n4_sse_html_escape2_aligned(buffer v142_buf,
+                            byteptr v141_ptr,
+                            nat v140_m,
+                            nat v139_nn)
+{
+  n4_sse_html_escape2_aligned:;
+  switch (sw_nat(v139_nn))
+  {
+    case_O_nat: { return n3_bufaddmem(v142_buf, v141_ptr, v140_m); }
+    case_S_nat: {
+      nat v144_nn_ = field0_S_nat(v139_nn);
+      byteptr v145_p1 = n2_bptradd(v141_ptr, v140_m);
+      m128 v146_bytes16 = n1_m128_of_bptr(v145_p1);
+      m128 v147_m = n0_chars_to_escape();
+      nat v148_n = n0_num_chars_to_escape();
+      nat v149_n = n0_O();
+      nat v150_n = n1_S(v149_n);
+      nat v151_n = n1_S(v150_n);
+      nat v152_n = n1_S(v151_n);
+      nat v153_n = n1_S(v152_n);
+      nat v154_n = n1_S(v153_n);
+      nat v155_n = n1_S(v154_n);
+      nat v156_n = n1_S(v155_n);
+      nat v157_n = n1_S(v156_n);
+      nat v158_n = n1_S(v157_n);
+      nat v159_n = n1_S(v158_n);
+      nat v160_n = n1_S(v159_n);
+      nat v161_n = n1_S(v160_n);
+      nat v162_n = n1_S(v161_n);
+      nat v163_n = n1_S(v162_n);
+      nat v164_n = n1_S(v163_n);
+      nat v165_n = n1_S(v164_n);
+      bool
+      v166_c
+      =
+      n4_cmpestrc_ubyte_eqany_ppol_lsig_bitmask(v147_m,
+      v148_n,
+      v146_bytes16,
+      v165_n);
+      m128 v167_m = n0_chars_to_escape();
+      nat v168_n = n0_num_chars_to_escape();
+      nat v169_n = n0_O();
+      nat v170_n = n1_S(v169_n);
+      nat v171_n = n1_S(v170_n);
+      nat v172_n = n1_S(v171_n);
+      nat v173_n = n1_S(v172_n);
+      nat v174_n = n1_S(v173_n);
+      nat v175_n = n1_S(v174_n);
+      nat v176_n = n1_S(v175_n);
+      nat v177_n = n1_S(v176_n);
+      nat v178_n = n1_S(v177_n);
+      nat v179_n = n1_S(v178_n);
+      nat v180_n = n1_S(v179_n);
+      nat v181_n = n1_S(v180_n);
+      nat v182_n = n1_S(v181_n);
+      nat v183_n = n1_S(v182_n);
+      nat v184_n = n1_S(v183_n);
+      nat v185_n = n1_S(v184_n);
+      m128
+      v186_b_
+      =
+      n4_cmpestrm_ubyte_eqany_ppol_lsig_bitmask(v167_m,
+      v168_n,
+      v146_bytes16,
+      v185_n);
+      switch (sw_bool(v166_c))
+      {
+        case_true_bool: {
+          nat v187_b = n1_lo64_of_m128(v186_b_);
+          buffer v188_buf1 = n3_bufaddmem(v142_buf, v141_ptr, v140_m);
+          nat v189_n = n0_O();
+          nat v190_n = n1_S(v189_n);
+          nat v191_n = n1_S(v190_n);
+          nat v192_n = n1_S(v191_n);
+          nat v193_n = n1_S(v192_n);
+          nat v194_n = n1_S(v193_n);
+          nat v195_n = n1_S(v194_n);
+          nat v196_n = n1_S(v195_n);
+          nat v197_n = n1_S(v196_n);
+          nat v198_n = n1_S(v197_n);
+          nat v199_n = n1_S(v198_n);
+          nat v200_n = n1_S(v199_n);
+          nat v201_n = n1_S(v200_n);
+          nat v202_n = n1_S(v201_n);
+          nat v203_n = n1_S(v202_n);
+          nat v204_n = n1_S(v203_n);
+          nat v205_n = n1_S(v204_n);
+          buffer
+          v206_buf2
+          =
+          n4_sse_html_escape2_dense(v188_buf1,
+          v205_n,
+          v187_b,
+          v146_bytes16);
+          nat v207_n = n0_O();
+          nat v208_n = n1_S(v207_n);
+          nat v209_n = n1_S(v208_n);
+          nat v210_n = n1_S(v209_n);
+          nat v211_n = n1_S(v210_n);
+          nat v212_n = n1_S(v211_n);
+          nat v213_n = n1_S(v212_n);
+          nat v214_n = n1_S(v213_n);
+          nat v215_n = n1_S(v214_n);
+          nat v216_n = n1_S(v215_n);
+          nat v217_n = n1_S(v216_n);
+          nat v218_n = n1_S(v217_n);
+          nat v219_n = n1_S(v218_n);
+          nat v220_n = n1_S(v219_n);
+          nat v221_n = n1_S(v220_n);
+          nat v222_n = n1_S(v221_n);
+          nat v223_n = n1_S(v222_n);
+          byteptr v224_b = n2_bptradd(v145_p1, v223_n);
+          nat v225_n = n0_O();
+          v142_buf = v206_buf2;
+          v141_ptr = v224_b;
+          v140_m = v225_n;
+          v139_nn = v144_nn_;
+          goto n4_sse_html_escape2_aligned;
+        }
+        case_false_bool: {
+          nat v226_n = n0_O();
+          nat v227_n = n1_S(v226_n);
+          nat v228_n = n1_S(v227_n);
+          nat v229_n = n1_S(v228_n);
+          nat v230_n = n1_S(v229_n);
+          nat v231_n = n1_S(v230_n);
+          nat v232_n = n1_S(v231_n);
+          nat v233_n = n1_S(v232_n);
+          nat v234_n = n1_S(v233_n);
+          nat v235_n = n1_S(v234_n);
+          nat v236_n = n1_S(v235_n);
+          nat v237_n = n1_S(v236_n);
+          nat v238_n = n1_S(v237_n);
+          nat v239_n = n1_S(v238_n);
+          nat v240_n = n1_S(v239_n);
+          nat v241_n = n1_S(v240_n);
+          nat v242_n = n1_S(v241_n);
+          nat v243_n = n2_addn(v140_m, v242_n);
+          v140_m = v243_n;
+          v139_nn = v144_nn_;
+          goto n4_sse_html_escape2_aligned;
+        }
+      }
+    }
+  }
+}
+buffer
+n3_sse_html_escape2(buffer v246_buf, byteptr v245_ptr, nat v244_n)
+{
+  nat v247_n = n0_O();
+  nat v248_n = n1_S(v247_n);
+  nat v249_n = n1_S(v248_n);
+  nat v250_n = n1_S(v249_n);
+  nat v251_n = n1_S(v250_n);
+  nat v252_n = n1_S(v251_n);
+  nat v253_n = n1_S(v252_n);
+  nat v254_n = n1_S(v253_n);
+  nat v255_n = n1_S(v254_n);
+  nat v256_n = n1_S(v255_n);
+  nat v257_n = n1_S(v256_n);
+  nat v258_n = n1_S(v257_n);
+  nat v259_n = n1_S(v258_n);
+  nat v260_n = n1_S(v259_n);
+  nat v261_n = n1_S(v260_n);
+  nat v262_n = n1_S(v261_n);
+  bool v263_b = n2_leq(v244_n, v262_n);
+  switch (sw_bool(v263_b))
+  {
+    case_true_bool: {
+      return n3_trec_html_escape(v246_buf, v245_ptr, v244_n);
+    }
+    case_false_bool: {
+      nat v264_n = n0_O();
+      nat v265_n = n1_S(v264_n);
+      nat v266_n = n1_S(v265_n);
+      nat v267_n = n1_S(v266_n);
+      nat v268_n = n1_S(v267_n);
+      nat v269_n = n1_S(v268_n);
+      nat v270_n = n1_S(v269_n);
+      nat v271_n = n1_S(v270_n);
+      nat v272_n = n1_S(v271_n);
+      nat v273_n = n1_S(v272_n);
+      nat v274_n = n1_S(v273_n);
+      nat v275_n = n1_S(v274_n);
+      nat v276_n = n1_S(v275_n);
+      nat v277_n = n1_S(v276_n);
+      nat v278_n = n1_S(v277_n);
+      nat v279_n = n1_S(v278_n);
+      nat v280_n = n1_S(v279_n);
+      nat v281_left_align = n2_align_of_bptr(v280_n, v245_ptr);
+      nat v282_left_len;
+      switch (sw_nat(v281_left_align))
+      {
+        case_O_nat: { v282_left_len = n0_O(); break; }
+        case_S_nat: {
+          nat v283_n = field0_S_nat(v281_left_align);
+          nat v284_n = n0_O();
+          nat v285_n = n1_S(v284_n);
+          nat v286_n = n1_S(v285_n);
+          nat v287_n = n1_S(v286_n);
+          nat v288_n = n1_S(v287_n);
+          nat v289_n = n1_S(v288_n);
+          nat v290_n = n1_S(v289_n);
+          nat v291_n = n1_S(v290_n);
+          nat v292_n = n1_S(v291_n);
+          nat v293_n = n1_S(v292_n);
+          nat v294_n = n1_S(v293_n);
+          nat v295_n = n1_S(v294_n);
+          nat v296_n = n1_S(v295_n);
+          nat v297_n = n1_S(v296_n);
+          nat v298_n = n1_S(v297_n);
+          nat v299_n = n1_S(v298_n);
+          nat v300_n = n1_S(v299_n);
+          v282_left_len = n2_subn(v300_n, v281_left_align);
+          break;
+        }
+      }
+      nat v301_notleft_len = n2_subn(v244_n, v282_left_len);
+      nat v302_n = n0_O();
+      nat v303_n = n1_S(v302_n);
+      nat v304_n = n1_S(v303_n);
+      nat v305_n = n1_S(v304_n);
+      nat v306_n = n1_S(v305_n);
+      nat v307_n = n1_S(v306_n);
+      nat v308_n = n1_S(v307_n);
+      nat v309_n = n1_S(v308_n);
+      nat v310_n = n1_S(v309_n);
+      nat v311_n = n1_S(v310_n);
+      nat v312_n = n1_S(v311_n);
+      nat v313_n = n1_S(v312_n);
+      nat v314_n = n1_S(v313_n);
+      nat v315_n = n1_S(v314_n);
+      nat v316_n = n1_S(v315_n);
+      nat v317_n = n1_S(v316_n);
+      nat v318_n = n1_S(v317_n);
+      nat v319_mid_count = n2_divn(v301_notleft_len, v318_n);
+      nat v320_n = n0_O();
+      nat v321_n = n1_S(v320_n);
+      nat v322_n = n1_S(v321_n);
+      nat v323_n = n1_S(v322_n);
+      nat v324_n = n1_S(v323_n);
+      nat v325_n = n1_S(v324_n);
+      nat v326_n = n1_S(v325_n);
+      nat v327_n = n1_S(v326_n);
+      nat v328_n = n1_S(v327_n);
+      nat v329_n = n1_S(v328_n);
+      nat v330_n = n1_S(v329_n);
+      nat v331_n = n1_S(v330_n);
+      nat v332_n = n1_S(v331_n);
+      nat v333_n = n1_S(v332_n);
+      nat v334_n = n1_S(v333_n);
+      nat v335_n = n1_S(v334_n);
+      nat v336_n = n1_S(v335_n);
+      nat v337_right_len = n2_modn(v301_notleft_len, v336_n);
+      buffer
+      v338_buf2
+      =
+      n4_sse_html_escape2_aligned(v246_buf,
+      v245_ptr,
+      v282_left_len,
+      v319_mid_count);
+      nat v339_n = n2_subn(v244_n, v337_right_len);
+      byteptr v340_b = n2_bptradd(v245_ptr, v339_n);
+      return n3_trec_html_escape(v338_buf2, v340_b, v337_right_len);
+    }
+  }
+}
